AReg.thy
@@ -6,7 +6,7 @@ section "Regexp definition and semantics"
 
 datatype ('v)regexp = ESet |(* EString |*) LChr 'v| Concat "'v regexp" "'v regexp"|
                       Alter "('v) regexp" "('v) regexp" (infix "||" 55) | Dot|
-                      Star "'v regexp" | Plus "('v) regexp"("_+") | Ques "('v) regexp"("_?")          
+                      Star "'v regexp" | Plus "('v) regexp"("_+") | Ques "('v) regexp"("_?") | \<epsilon>         
 
 inductive_set star :: "'v list set \<Rightarrow> 'v list set" 
   for r :: "'v list set" where
@@ -14,18 +14,17 @@ zero[intro!]:"[] \<in> star r"|
 step[intro!]:"x \<in> r \<and> y \<in> star r \<Longrightarrow> x@y \<in> star r"
 
 primrec sem_reg :: "('v) regexp => 'v set\<Rightarrow> 'v list set" where 
-"sem_reg ESet v = {[]}"| (*Empty Set*)
+"sem_reg ESet v = {}"| (*Empty Set*)
 (*"sem_reg EString v = {[]}"| (*Empty String*)*)
-"sem_reg (Dot) vset = (if vset = {} then {[]} else (λu. [u]) ` vset)" | 
+"sem_reg (Dot) vset = (λu. [u]) ` vset" | 
 "sem_reg (Concat r1 r2) v =(λu. fst u @ snd u) ` (sem_reg r1 v × sem_reg r2 v)"|
 "sem_reg (LChr a) v = {[a]}"|
 "sem_reg (v1||v2) a = (sem_reg v1 a) \<union> (sem_reg v2 a)"|
 "sem_reg (Star a) v = star (sem_reg a v)"|
 "sem_reg (Plus a) v = (sem_reg a v) \<union> star (sem_reg a v)  "|
-"sem_reg (Ques v) a = {[]} \<union> (sem_reg v a)"
+"sem_reg (Ques v) a = {[]} \<union> (sem_reg v a)"|
+"sem_reg \<epsilon> v = {[]}"
 
-fun f ::"'v set \<Rightarrow> 'v set\<Rightarrow> ('v * 'v)set" where
-"f s1 s2 = {(x,y). x \<in> s1 \<and> y \<in> s2}" 
 
 primrec  alp_reg :: "'v regexp \<Rightarrow> 'v set \<Rightarrow> 'v set" where
 "alp_reg (LChr n) vs=  {n}"|
@@ -36,6 +35,7 @@ primrec  alp_reg :: "'v regexp \<Rightarrow> 'v set \<Rightarrow> 'v set" where
 "alp_reg (Dot) vs = vs"|
 "alp_reg (Star v) vs = alp_reg v vs"| 
 "alp_reg (Plus v) vs = alp_reg v vs"|
-"alp_reg (Ques v) vs = alp_reg v vs"
+"alp_reg (Ques v) vs = alp_reg v vs"|
+"alp_reg \<epsilon> vs = {}"
 
 end
